rename T to lst

Sepreftime.thy
@@ -766,7 +766,7 @@ term REST
 
 
 
-section \<open>T - Generalized Weakest Precondition\<close>
+section \<open>Generalized Weakest Precondition\<close>
 
 subsection "mm"
 
@@ -904,17 +904,17 @@ lemma mii_inf: "mii Qf M x = Some \<infinity> \<longleftrightarrow> (\<exists>Mf
 lemma miiFailt: "mii Q FAILT x = None" unfolding mii_def by auto
 
 
-subsection "T"
+subsection "lst - latest starting time"
 
-definition T :: "('a \<Rightarrow> enat option) \<Rightarrow> 'a nrest \<Rightarrow> enat option" 
-  where "T Qf M =  Inf { mii Qf M x | x. True}"
+definition lst :: "('a \<Rightarrow> enat option) \<Rightarrow> 'a nrest \<Rightarrow> enat option" 
+  where "lst Qf M =  Inf { mii Qf M x | x. True}"
 
-lemma T_alt_: "T Qf M = Inf ( (mii Qf M) ` UNIV )"
-  unfolding T_def 
+lemma T_alt_: "lst Qf M = Inf ( (mii Qf M) ` UNIV )"
+  unfolding lst_def 
   by (simp add: full_SetCompr_eq) 
 
-lemma T_pw: "T Q M \<ge> t \<longleftrightarrow> (\<forall>x. mii Q M x \<ge> t)"
-  unfolding T_def mii_def apply(cases M) apply auto
+lemma T_pw: "lst Q M \<ge> t \<longleftrightarrow> (\<forall>x. mii Q M x \<ge> t)"
+  unfolding lst_def mii_def apply(cases M) apply auto
   unfolding Inf_option_def apply (auto split: if_splits)
   using less_eq_option_None_is_None less_option_None not_less apply blast
   apply (smt Inf_lower Inf_option_def dual_order.trans mem_Collect_eq)
@@ -923,7 +923,7 @@ lemma T_pw: "T Q M \<ge> t \<longleftrightarrow> (\<forall>x. mii Q M x \<ge> t)
   
 
 
-lemma z: "(\<forall>t. T Q M \<ge> t \<longrightarrow> T Q' M' \<ge> t) \<Longrightarrow> T Q M \<le> T Q' M'"
+lemma z: "(\<forall>t. lst Q M \<ge> t \<longrightarrow> lst Q' M' \<ge> t) \<Longrightarrow> lst Q M \<le> lst Q' M'"
   by simp
 
 (*
@@ -996,16 +996,16 @@ lemma pw_bindT_nofailT_2[refine_pw_simps]: "nofailT (bindT M f) \<longleftrighta
 
 lemma kla: "M = SPECT Mff \<Longrightarrow> inres2 M x = (Mff x \<noteq> None)" unfolding inres2_def by (auto split: nrest.splits)
 
-lemma "M = FAILi \<Longrightarrow> T Q M = None" unfolding T_def by (auto simp: mii_def)
+lemma "M = FAILi \<Longrightarrow> T Q M = None" unfolding lst_def by (auto simp: mii_def)
 
 lemma fall2: "M = REST Mf \<Longrightarrow> Mf x = Some t \<Longrightarrow> Q x = None \<Longrightarrow> T Q M = None"
-  unfolding T_def
+  unfolding lst_def
   apply(rule None_in_Inf)
   apply (auto simp: mii_def mm_def)
   apply(rule exI[where x=x]) by auto  
 
 lemma fall3: "M = REST Mf \<Longrightarrow> Mf x = Some t \<Longrightarrow> Q x = Some t' \<Longrightarrow> t' < t \<Longrightarrow> T Q M = None"
-  unfolding T_def
+  unfolding lst_def
   apply(rule None_in_Inf)
   apply (auto simp: mii_def mm_def)
   apply(rule exI[where x=x]) by auto 
@@ -1018,11 +1018,11 @@ lemma k2: "None = Inf S \<longleftrightarrow> (None \<in> S)"
 lemma T_None_char: "T Q M = None \<longleftrightarrow> (M = FAILi \<or> (\<exists>Mf t x. M = REST Mf \<and> Mf x = Some t \<and> (Q x = None \<or> (\<exists>t'. Q x = Some t' \<and> t'<t))))"
   apply rule
   subgoal
-    unfolding T_def k
+    unfolding lst_def k
     apply auto
     apply(cases M) apply (auto simp: mii_def mm_def split: option.splits) by force
   subgoal
-    unfolding T_def
+    unfolding lst_def
     apply(rule None_in_Inf) 
     apply (auto simp: mii_def mm_def split: option.splits ) apply force+  
     done
@@ -1042,10 +1042,10 @@ lemma assumes "T Q M = Some (enat t)"
   shows T_SomeEnat: "(\<exists>Mf. M = REST Mf \<and> (\<exists>x t' t'' . Mf x = Some (enat t') \<and> Q x = Some (enat t'') \<and> t = t''-t' \<and> t''\<ge>t')
                            \<and> (\<forall>x t' t''. Mf x = Some (enat t') \<and> Q x = Some (enat t'') \<and> t''\<ge>t' \<longrightarrow> t \<le> t''-t' ))"
 proof -
-  from assms have "(LEAST t. t \<in> {mii Q M x |x. True}) = Some (enat t)" unfolding T_def using tz by metis
+  from assms have "(LEAST t. t \<in> {mii Q M x |x. True}) = Some (enat t)" unfolding lst_def using tz by metis
   then have 1: "Some (enat t)\<in> {mii Q M x |x. True}" and 2: "\<forall>e\<in>{mii Q M x |x. True}. e\<ge> Some (enat t)"
     apply (metis (mono_tags, lifting) LeastI_ex mem_Collect_eq)
-    by (metis (mono_tags) Inf_lower T_def \<open>T Q M = Some (enat t)\<close>)  
+    by (metis (mono_tags) Inf_lower lst_def \<open>T Q M = Some (enat t)\<close>)  
 
 
   from 1 have "\<exists>x. mii Q M x = Some (enat t)" by auto
@@ -1083,19 +1083,19 @@ definition nres3 where "nres3 Q M x t \<longleftrightarrow> mii Q M x \<ge> t"
 
 lemma pw_T_le:
   assumes "\<And>t. (\<forall>x. nres3 Q M x t) \<Longrightarrow> (\<forall>x. nres3 Q' M' x t)"
-  shows "T Q M \<le> T Q' M'"
+  shows "lst Q M \<le> lst Q' M'"
   apply(rule z)
   using assms unfolding T_pw nres3_def  by metis 
 
 lemma assumes "\<And>t. (\<forall>x. nres3 Q M x t) = (\<forall>x. nres3 Q' M' x t)" 
-  shows pw_T_eq_iff: "T Q M = T Q' M'"
+  shows pw_T_eq_iff: "lst Q M = lst Q' M'"
   apply (rule antisym)
   apply(rule pw_T_le) using assms apply metis
   apply(rule pw_T_le) using assms apply metis done 
 
 lemma assumes "\<And>t. (\<forall>x. nres3 Q M x t) \<Longrightarrow> (\<forall>x. nres3 Q' M' x t)"
       "\<And>t. (\<forall>x. nres3 Q' M' x t) \<Longrightarrow> (\<forall>x. nres3 Q M x t)"
-  shows pw_T_eqI: "T Q M = T Q' M'"
+  shows pw_T_eqI: "lst Q M = lst Q' M'"
   apply (rule antisym)
   apply(rule pw_T_le) apply fact
   apply(rule pw_T_le) apply fact done 
@@ -1171,32 +1171,29 @@ proof -
 qed
 
 
-lemma nres3_bindT: "(\<forall>x. nres3 Q (bindT m f) x t) = (\<forall>y. nres3 (\<lambda>y. T Q (f y)) m y t)"
+lemma nres3_bindT: "(\<forall>x. nres3 Q (bindT m f) x t) = (\<forall>y. nres3 (\<lambda>y. lst Q (f y)) m y t)"
 proof -
   have "(\<forall>x. nres3 Q (bindT m f) x t) = (\<forall>x.  t \<le> mii Q (bindT m f) x)" unfolding nres3_def by auto
   also have "\<dots> = (\<forall>x. (\<forall>y. t \<le> mii (\<lambda>y. mii Q (f y) x) m y))" by(simp only: mii_bindT)
   also have "\<dots> = (\<forall>y. (\<forall>x. t \<le> mii (\<lambda>y. mii Q (f y) x) m y))" by blast
   also have "\<dots> = (\<forall>y.  t \<le> mii (\<lambda>y. Inf {mii Q (f y) x|x. True}) m y)" 
     apply(simp only: mii_continuous) using t by fast
-  also have "\<dots> = (\<forall>y.  t \<le> mii (\<lambda>y. T Q (f y)) m y)" unfolding T_def by auto
-  also have "\<dots> = (\<forall>y. nres3 (\<lambda>y. T Q (f y)) m y t)" unfolding nres3_def by auto
+  also have "\<dots> = (\<forall>y.  t \<le> mii (\<lambda>y. lst Q (f y)) m y)" unfolding lst_def by auto
+  also have "\<dots> = (\<forall>y. nres3 (\<lambda>y. lst Q (f y)) m y t)" unfolding nres3_def by auto
   finally show ?thesis .
-  have "(\<forall>y.  t \<le> mii (\<lambda>y. T Q (f y)) m y) = (t \<le> Inf{ mii (\<lambda>y. T Q (f y)) m y|y. True})" using t by metis
+  have "(\<forall>y.  t \<le> mii (\<lambda>y. lst Q (f y)) m y) = (t \<le> Inf{ mii (\<lambda>y. lst Q (f y)) m y|y. True})" using t by metis
 qed
 
 
 subsection "rules for T"
 
-lemma T_bindT: "T Q (bindT M f) = T (\<lambda>y. T Q (f y)) M"
+lemma T_bindT: "lst Q (bindT M f) = lst (\<lambda>y. lst Q (f y)) M"
   by (rule pw_T_eq_iff, rule nres3_bindT)
 
-
-definition "lst c Q = (\<lambda>s. T Q (c s))"
-lemma "lst (%x. bindT (M x) f) Q = lst M (lst f Q)"
-  unfolding lst_def apply rule by (simp only: T_bindT) 
+  
 
 
-lemma T_REST: "T Q (REST [x\<mapsto>t]) = mm2 (Q x) (Some t)"
+lemma T_REST: "lst Q (REST [x\<mapsto>t]) = mm2 (Q x) (Some t)"
 proof- 
   have *: "Inf {uu. \<exists>xa. (xa = x \<longrightarrow> uu= v) \<and> (xa \<noteq> x \<longrightarrow> uu = Some \<infinity>)} = v"  (is "Inf ?S = v") for v :: "enat option"
   proof -
@@ -1204,11 +1201,11 @@ proof-
     then show ?thesis apply simp apply safe by (simp_all add: top_enat_def[symmetric] top_option_def[symmetric] ) 
   qed
   then show ?thesis
-    unfolding T_def mii_alt by auto
+    unfolding lst_def mii_alt by auto
 qed
 
 
-lemma T_RETURNT: "T Q (RETURNT x) = Q x"
+lemma T_RETURNT: "lst Q (RETURNT x) = Q x"
   unfolding RETURNT_alt apply(rule trans) apply(rule T_REST) by simp
                 
 thm T_pw
@@ -1244,29 +1241,29 @@ lemma aux1a': "(\<forall>t''. Q' = Some t'' \<longrightarrow> (Q) \<ge> Some (t 
   subgoal for t'' using aux1 by metis
   done
 
-lemma "T Q (SPECT P) \<ge> Some t \<longleftrightarrow> (\<forall>x t'. P x = Some t' \<longrightarrow> (Q x \<ge> Some (t + t')))"
+lemma "lst Q (SPECT P) \<ge> Some t \<longleftrightarrow> (\<forall>x t'. P x = Some t' \<longrightarrow> (Q x \<ge> Some (t + t')))"
   apply (auto simp: T_pw mii_alt)
   apply (metis aux1)
   apply (simp add: aux1a'[symmetric])
   done
 
 
-lemma "T Q (SPECT P) \<ge> Some t \<longleftrightarrow> (\<forall>x t'. P x = Some t' \<longrightarrow> (\<exists>t''. Q x = Some t'' \<and> t'' \<ge> t + t'))"
+lemma "lst Q (SPECT P) \<ge> Some t \<longleftrightarrow> (\<forall>x t'. P x = Some t' \<longrightarrow> (\<exists>t''. Q x = Some t'' \<and> t'' \<ge> t + t'))"
   apply (auto simp: T_pw mii_alt )
    apply (metis aux1 le_some_optE)
   apply (simp add: aux1a'[symmetric])
   apply auto 
   by fastforce
 
-lemma "T Q (SPECT P) = Some t \<longleftrightarrow> (\<forall>x t'. P x = Some t' \<longrightarrow> (\<exists>t''. Q x = Some t'' \<and> t'' = t + t'))"
-  apply (auto simp: T_def ) oops
+lemma "lst Q (SPECT P) = Some t \<longleftrightarrow> (\<forall>x t'. P x = Some t' \<longrightarrow> (\<exists>t''. Q x = Some t'' \<and> t'' = t + t'))"
+  apply (auto simp: lst_def ) oops
 
 
 lemma T_SELECT: 
   assumes  
-    "\<forall>x. \<not> P x \<Longrightarrow> Some tt \<le> T Q (SPECT [None \<mapsto> tf])"
-  and p: "(\<And>x. P x \<Longrightarrow> Some tt \<le> T Q (SPECT [Some x \<mapsto> tf]))"
-   shows "Some tt \<le> T Q (SELECT P tf)"
+    "\<forall>x. \<not> P x \<Longrightarrow> Some tt \<le> lst Q (SPECT [None \<mapsto> tf])"
+  and p: "(\<And>x. P x \<Longrightarrow> Some tt \<le> lst Q (SPECT [Some x \<mapsto> tf]))"
+   shows "Some tt \<le> lst Q (SELECT P tf)"
 proof(cases "\<exists>x. P x")
   case True
   from p[unfolded T_pw mii_alt] have
@@ -1305,9 +1302,9 @@ lemma aux1': "Some t \<le> mm2 Q (Some t') \<longleftrightarrow> Some (t+t') \<l
 
 lemma T_conseq4:
   assumes 
-    "T Q' f \<ge> Some t'"
+    "lst Q' f \<ge> Some t'"
     "\<And>x t'' M. Q' x = Some t'' \<Longrightarrow> (Q x) \<ge> Some ((t - t') + t'')" 
-  shows "T Q f \<ge> Some t"
+  shows "lst Q f \<ge> Some t"
 proof -
   {
     fix x
@@ -1336,7 +1333,7 @@ lemma T_conseq44:
   shows "T Q f \<ge> Some t"
 proof -
   { assume "T Q f = Some \<infinity>"
-    then have "False" unfolding T_def 
+    then have "False" unfolding lst_def 
 
   {
     fix x
@@ -1361,9 +1358,9 @@ qed*)
 
 lemma T_conseq6:
   assumes 
-    "T Q' f \<ge> Some t"
+    "lst Q' f \<ge> Some t"
     "\<And>x t'' M. f = SPECT M \<Longrightarrow> M x \<noteq> None \<Longrightarrow> Q' x = Some t'' \<Longrightarrow> (Q x) \<ge> Some ( t'')" 
-  shows "T Q f \<ge> Some t"
+  shows "lst Q f \<ge> Some t"
 proof -
   {
     fix x
@@ -1389,18 +1386,18 @@ qed
 
 lemma T_conseq6':
   assumes 
-    "T Q' f \<ge> Some t"
+    "lst Q' f \<ge> Some t"
     "\<And>x t'' M. f = SPECT M \<Longrightarrow> M x \<noteq> None \<Longrightarrow>   (Q x) \<ge> Q' x" 
-  shows "T Q f \<ge> Some t"
+  shows "lst Q f \<ge> Some t"
   apply(rule T_conseq6) apply fact   
      by (auto dest: assms(2))
 
 
 lemma T_conseq5:
   assumes 
-    "T Q' f \<ge> Some t'"
+    "lst Q' f \<ge> Some t'"
     "\<And>x t'' M. f = SPECT M \<Longrightarrow> M x \<noteq> None \<Longrightarrow> Q' x = Some t'' \<Longrightarrow> (Q x) \<ge> Some ((t - t') + t'')" 
-  shows "T Q f \<ge> Some t"
+  shows "lst Q f \<ge> Some t"
 proof -
   {
     fix x
@@ -1425,9 +1422,9 @@ qed
 
 lemma T_conseq3: 
   assumes 
-    "T Q' f \<ge> Some t'"
+    "lst Q' f \<ge> Some t'"
     "\<And>x. mm2 (Q x) (Q' x) \<ge> Some (t - t')" 
-  shows "T Q f \<ge> Some t"
+  shows "lst Q f \<ge> Some t"
   using assms T_conseq4 aux1a by metis
 
 
@@ -1442,10 +1439,10 @@ method vcg uses rls = ((rule rls vcg_rules[THEN T_conseq4] | clarsimp simp: emb_
 
 
 lemma assumes
-  f_spec[vcg_rules]: "T ( emb' (\<lambda>x. x > 2) (enat o (( *) 2)) ) f \<ge> Some 0"
+  f_spec[vcg_rules]: "lst ( emb' (\<lambda>x. x > 2) (enat o (( *) 2)) ) f \<ge> Some 0"
 and 
-  g_spec[vcg_rules]: "T ( emb' (\<lambda>x. x > 2) (enat) ) g \<ge> Some 0"
-shows "T ( emb' (\<lambda>x. x > 5) (enat o ( *) 3) ) (P f g) \<ge> Some 0"
+  g_spec[vcg_rules]: "lst ( emb' (\<lambda>x. x > 2) (enat) ) g \<ge> Some 0"
+shows "lst ( emb' (\<lambda>x. x > 5) (enat o ( *) 3) ) (P f g) \<ge> Some 0"
 proof -
   have ?thesis
     unfolding P_def
@@ -1471,7 +1468,7 @@ hide_const P
 
 
 
-find_theorems "T _ _ \<ge> _"
+find_theorems "lst _ _ \<ge> _"
 
 lemma [simp]: "mm2 None q = (case q of None \<Rightarrow> Some \<infinity> | _ \<Rightarrow> None)"
   apply (cases q) apply (auto simp: mm2_def) done
@@ -1489,7 +1486,7 @@ lemma auxXX1: "Some t \<le> mm2 (Q x) (Some t') \<Longrightarrow> Some t' \<le> 
   done
 
 
-definition "TSPEC Q m \<equiv> T Q m \<ge> Some 0"
+definition "TSPEC Q m \<equiv> lst Q m \<ge> Some 0"
 
 lemma "TSPEC Q m \<longleftrightarrow> (case m of FAILi \<Rightarrow> False | REST M \<Rightarrow> 
   \<forall>x. mm2 (Q x) (M x) \<ge> Some 0
@@ -1497,7 +1494,7 @@ lemma "TSPEC Q m \<longleftrightarrow> (case m of FAILi \<Rightarrow> False | RE
   by (auto simp: T_pw TSPEC_def mii_alt split: option.splits nrest.splits)
 
 
-lemma fold_TSPEC: "T Q m \<ge> Some t \<longleftrightarrow> TSPEC (\<lambda>x. mm2 (Q x) (Some t)) m"
+lemma fold_TSPEC: "lst Q m \<ge> Some t \<longleftrightarrow> TSPEC (\<lambda>x. mm2 (Q x) (Some t)) m"
   apply (auto simp: TSPEC_def T_pw mii_alt split: option.splits nrest.splits simp: aux1a'[where t=0, symmetric, simplified])
 
   subgoal for x
@@ -1517,33 +1514,33 @@ lemma fold_TSPEC: "T Q m \<ge> Some t \<longleftrightarrow> TSPEC (\<lambda>x. m
 lemma enat_minus_mono: "a' \<ge> b \<Longrightarrow> a' \<ge> a \<Longrightarrow> a' - b \<ge> (a::enat) - b"
   apply(cases a; cases b; cases a') by auto
 
-lemma waux1: "(\<forall>s t'. I s = Some t' \<longrightarrow> b s  \<longrightarrow> c s \<noteq> FAILi \<and>  T (Q s) (c s) \<ge> Some t')
-    = (T (\<lambda>s. T (Q s) (c s)) (SPECT (\<lambda>x. if b x then I x else None)) \<ge> Some 0)"
+lemma waux1: "(\<forall>s t'. I s = Some t' \<longrightarrow> b s  \<longrightarrow> c s \<noteq> FAILi \<and>  lst (Q s) (c s) \<ge> Some t')
+    = (lst (\<lambda>s. lst (Q s) (c s)) (SPECT (\<lambda>x. if b x then I x else None)) \<ge> Some 0)"
   apply(subst (2)T_pw) unfolding mii_alt apply simp
   apply (auto simp: mm2_def split: option.splits)
   subgoal by force  
   subgoal by force
-  subgoal by (simp add: T_def miiFailt)
-  subgoal by (metis (no_types, lifting) Inf_option_def T_def leI less_option_Some)
+  subgoal by (simp add: lst_def miiFailt)
+  subgoal by (metis (no_types, lifting) Inf_option_def lst_def leI less_option_Some)
   done  
 
 
-lemma waux2: "(\<forall>s t'. I s = Some t' \<longrightarrow> T (\<lambda>x. if b x then None else I x) (whileT b c s) \<ge> Some t')
-      = (T (\<lambda>s. T (\<lambda>x. if b x then None else I x) (whileT b c s)) (SPECT I) \<ge> Some 0)"  
+lemma waux2: "(\<forall>s t'. I s = Some t' \<longrightarrow> lst (\<lambda>x. if b x then None else I x) (whileT b c s) \<ge> Some t')
+      = (lst (\<lambda>s. lst (\<lambda>x. if b x then None else I x) (whileT b c s)) (SPECT I) \<ge> Some 0)"  
   apply(subst (2) T_pw) unfolding mii_alt apply simp
   by (force simp: mm2_def split: option.splits)  
 
-lemma T_ineq_D: "Some t' \<le> T I (c x) \<Longrightarrow> (\<exists>M. c x = SPECT M \<and> mm2 (I y) (M y)  \<ge> Some t')"
+lemma T_ineq_D: "Some t' \<le> lst I (c x) \<Longrightarrow> (\<exists>M. c x = SPECT M \<and> mm2 (I y) (M y)  \<ge> Some t')"
   unfolding T_pw mii_alt apply (auto split: nrest.splits) using nrest_noREST_FAILT by blast 
 
 
 lemma
   assumes "whileT b c s = r"
-  assumes IS: "\<And>s t'. I s = Some t' \<Longrightarrow> b s  \<Longrightarrow> c s \<noteq> FAILi \<and>  T I (c s) \<ge> Some t'"
+  assumes IS: "\<And>s t'. I s = Some t' \<Longrightarrow> b s  \<Longrightarrow> c s \<noteq> FAILi \<and>  lst I (c s) \<ge> Some t'"
     (*  "T (\<lambda>x. T I (c x)) (SPECT (\<lambda>x. if b x then I x else None)) \<ge> Some 0" *) 
   assumes "I s = Some t'"
   assumes wf: "wf {(y, x)|x M y. I x \<noteq> None \<and> b x \<and> c x = SPECT M \<and> M y \<noteq> None}"
-  shows whileT_rule: "T (\<lambda>x. if b x then None else I x) r \<ge> Some t'"
+  shows whileT_rule: "lst (\<lambda>x. if b x then None else I x) r \<ge> Some t'"
   using assms(1,3)
   unfolding whileT_def
 proof (induction arbitrary: t' rule: RECT_wf_induct[where R="{(y, x)|x M y. I x \<noteq> None \<and> b x \<and> c x = SPECT M \<and> M y \<noteq> None}"])
@@ -1556,17 +1553,17 @@ next
   case step: (3 x D r t')
 
   { assume b:"b x"
-    with  IS step(3) have pff: "Some t' \<le> T I (c x)" and cnofail: "c x \<noteq> FAILi" by auto
+    with  IS step(3) have pff: "Some t' \<le> lst I (c x)" and cnofail: "c x \<noteq> FAILi" by auto
     from b step(2) have r: "r = bindT (c x) D" by auto
     from cnofail obtain M where cM: "c x = SPECT M" by force
 
-    from step(3) pff have inf: "I x \<le> T I (c x)" by auto
+    from step(3) pff have inf: "I x \<le> lst I (c x)" by auto
 
     have k: "\<And>y. M y \<noteq> None \<Longrightarrow> I y \<noteq> None"
       using inf[unfolded T_pw cM mii_alt] by (auto simp: mm2_def step(3) split: option.splits) 
 
     { fix y t''
-      have " None \<noteq> M y \<Longrightarrow> I y = Some t'' \<Longrightarrow> Some t'' \<le> T (\<lambda>x. if b x then None else I x) (D y)"
+      have " None \<noteq> M y \<Longrightarrow> I y = Some t'' \<Longrightarrow> Some t'' \<le> lst (\<lambda>x. if b x then None else I x) (D y)"
         apply(rule step(1)[where y=y])
         subgoal apply auto subgoal using step(3) by auto subgoal using b by simp apply(rule exI[where x=M]) using cM  
           using leI by fastforce          
@@ -1578,18 +1575,18 @@ next
       from step(3) inf have pot_pays: "\<And>y. I x \<le> mm2 (I y) (M y)" unfolding T_pw mii_alt using cM by (auto split: nrest.splits)
       from pot_pays have ineq: "I x \<le> mm2 (I y) (M y)" by auto 
 
-      have " Some t' \<le> mii (\<lambda>y. T (\<lambda>x. if b x then None else I x) (D y)) (c x) y" 
+      have " Some t' \<le> mii (\<lambda>y. lst (\<lambda>x. if b x then None else I x) (D y)) (c x) y" 
         unfolding mii_alt using cM apply(auto split: nrest.splits) 
         unfolding mm2_def apply (auto split: option.splits)
         subgoal using pf  
-          by (metis (no_types, lifting) Inf_option_def RETURNT_alt T_RETURNT T_def k less_eq_option_Some_None option.distinct(1))
+          by (metis (no_types, lifting) Inf_option_def RETURNT_alt T_RETURNT lst_def k less_eq_option_Some_None option.distinct(1))
       proof - 
         fix th tn  (* time that we have, time that we need *)
-        assume  My: "M y = Some tn" and T: "T (\<lambda>x. if b x then None else I x) (D y) = Some th" 
+        assume  My: "M y = Some tn" and T: "lst (\<lambda>x. if b x then None else I x) (D y) = Some th" 
 
         from ineq obtain tiy where Iy: "I y = Some tiy" using My step(3) by(auto simp: mm2_def split: if_splits option.splits)
         with ineq My step(3) have 2: "tiy \<ge> tn" and a2: "t' \<le> tiy - tn" by (auto simp: mm2_def split: if_splits) 
-        from cM My pf have "Some tiy \<le> T (\<lambda>x. if b x then None else I x) (D y)" by (simp add: \<open>I y = Some tiy\<close>)
+        from cM My pf have "Some tiy \<le> lst (\<lambda>x. if b x then None else I x) (D y)" by (simp add: \<open>I y = Some tiy\<close>)
         with T have 3: "tiy \<le> th" by simp
 
         { assume less: "th < tn"
@@ -1603,7 +1600,7 @@ next
         } 
       qed 
     }
-    then have "Some t' \<le> T (\<lambda>x. if b x then None else I x) (bindT (c x) D)"
+    then have "Some t' \<le> lst (\<lambda>x. if b x then None else I x) (bindT (c x) D)"
       apply(simp add: T_bindT) unfolding T_pw by auto
     then have ?case unfolding r by auto
   }
@@ -1644,7 +1641,7 @@ qed
 named_theorems vcg_simp_rules
 lemmas [vcg_simp_rules] = (* T_bindT *) T_RETURNT
 
-lemma TbindT_I: "Some t \<le>  T (\<lambda>y. T Q (f y)) M \<Longrightarrow>  Some t \<le> T Q (M \<bind> f)"
+lemma TbindT_I: "Some t \<le>  lst (\<lambda>y. lst Q (f y)) M \<Longrightarrow>  Some t \<le> lst Q (M \<bind> f)"
   by(simp add: T_bindT)
 
 method vcg' uses rls = ((rule rls TbindT_I vcg_rules[THEN T_conseq6] | clarsimp split: if_splits simp:  vcg_simp_rules)+)
@@ -1652,11 +1649,11 @@ method vcg' uses rls = ((rule rls TbindT_I vcg_rules[THEN T_conseq6] | clarsimp 
 lemma
   assumes "whileT b c s = r"
   assumes IS[vcg_rules]: "\<And>s t'. I s = Some t' \<Longrightarrow> b s 
-           \<Longrightarrow>    T (\<lambda>s'. if (s',s)\<in>R then I s' else None) (c s) \<ge> Some t'"
+           \<Longrightarrow>    lst (\<lambda>s'. if (s',s)\<in>R then I s' else None) (c s) \<ge> Some t'"
     (*  "T (\<lambda>x. T I (c x)) (SPECT (\<lambda>x. if b x then I x else None)) \<ge> Some 0" *) 
   assumes "I s = Some t"
   assumes wf: "wf R"
-  shows whileT_rule'': "T (\<lambda>x. if b x then None else I x) r \<ge> Some t"
+  shows whileT_rule'': "lst (\<lambda>x. if b x then None else I x) r \<ge> Some t"
   using assms(1,3)
   unfolding whileT_def
 proof (induction arbitrary: t rule: RECT_wf_induct[where R="R"])
@@ -1681,12 +1678,12 @@ qed
 lemma
   assumes "whileT b c s = r"
   assumes IS[vcg_rules]: "\<And>s t'. I s = Some t' \<Longrightarrow> b s 
-           \<Longrightarrow>    T (\<lambda>s'. if (s',s)\<in>R then I s' else None) (c s) \<ge> Some t'"
+           \<Longrightarrow>    lst (\<lambda>s'. if (s',s)\<in>R then I s' else None) (c s) \<ge> Some t'"
     (*  "T (\<lambda>x. T I (c x)) (SPECT (\<lambda>x. if b x then I x else None)) \<ge> Some 0" *) 
   assumes "I s = Some t"
   assumes wf: "wf R"
   assumes exit: "\<And>s t'. I s = Some t' \<Longrightarrow> \<not>b s \<Longrightarrow> Q s \<ge> Some t'"
-  shows whileT_rule''a_: "T Q r \<ge> Some t"
+  shows whileT_rule''a_: "lst Q r \<ge> Some t"
   using assms(1,3)
   unfolding whileT_def
 proof (induction arbitrary: t rule: RECT_wf_induct[where R="R"])
@@ -1722,8 +1719,8 @@ lemma mm3_Some_conv: "(mm3 t0 A = Some t) = (\<exists>t'. A = Some t' \<and> t0 
 
 lemma [simp]: "mm3 t0 None = None" unfolding mm3_def by auto
 
-lemma T_FAILT[simp]: "T Q FAILT = None"
-  unfolding T_def mii_alt by simp
+lemma T_FAILT[simp]: "lst Q FAILT = None"
+  unfolding lst_def mii_alt by simp
 
 definition "progress m \<equiv> \<forall>s' M. m = SPECT M \<longrightarrow> M s' \<noteq> None \<longrightarrow> M s' > Some 0"
 lemma progressD: "progress m \<Longrightarrow> m=SPECT M \<Longrightarrow> M s' \<noteq> None \<Longrightarrow> M s' > Some 0"
@@ -1805,11 +1802,11 @@ lemma
   assumes "whileT b c s0 = r"
   assumes progress: "\<And>s. progress (c s)" 
   assumes IS[vcg_rules]: "\<And>s t t'. I s = Some t \<Longrightarrow>  b s  \<Longrightarrow> 
-           T (\<lambda>s'. mm3 t (I s') ) (c s) \<ge> Some 0"
+           lst (\<lambda>s'. mm3 t (I s') ) (c s) \<ge> Some 0"
     (*  "T (\<lambda>x. T I (c x)) (SPECT (\<lambda>x. if b x then I x else None)) \<ge> Some 0" *) 
   assumes [simp]: "I s0 = Some t0" 
     (*  assumes wf: "wf R" *)                         
-  shows whileT_rule''': "T (\<lambda>x. if b x then None else mm3 t0 (I x)) r \<ge> Some 0"  
+  shows whileT_rule''': "lst (\<lambda>x. if b x then None else mm3 t0 (I x)) r \<ge> Some 0"  
   apply(rule T_conseq4)
    apply(rule whileT_rule''[where I="\<lambda>s. mm3 t0 (I s)"
         and R="measure (the_enat o the o I)", OF assms(1)])
@@ -1847,10 +1844,10 @@ lemma  whileIET_rule[THEN T_conseq6, vcg_rules]:
   assumes 
     "(\<And>s t t'.
     (if I s then Some (E s) else None) = Some t \<Longrightarrow>
-    b s \<Longrightarrow> Some 0 \<le> T (\<lambda>s'. mm3 t (if I s' then Some (E s') else None)) (C s))" 
+    b s \<Longrightarrow> Some 0 \<le> lst (\<lambda>s'. mm3 t (if I s' then Some (E s') else None)) (C s))" 
   "\<And>s. progress (C s)"
   "I s0" 
-shows "Some 0 \<le> T (\<lambda>x. if b x then None else mm3 (E s0) (if I x then Some (E x) else None)) (whileIET I E b C s0)"
+shows "Some 0 \<le> lst (\<lambda>x. if b x then None else mm3 (E s0) (if I x then Some (E x) else None)) (whileIET I E b C s0)"
   unfolding whileIET_def  
   apply(rule whileT_rule'''[OF refl, where I="(\<lambda>e. if I e
                 then Some (E e) else None)"])
@@ -1859,10 +1856,10 @@ shows "Some 0 \<le> T (\<lambda>x. if b x then None else mm3 (E s0) (if I x then
  
 
 lemma transf:
-  assumes "I s \<Longrightarrow>  b s \<Longrightarrow> Some 0 \<le> T (\<lambda>s'. mm3 (E s) (if I s' then Some (E s') else None)) (C s)" 
+  assumes "I s \<Longrightarrow>  b s \<Longrightarrow> Some 0 \<le> lst (\<lambda>s'. mm3 (E s) (if I s' then Some (E s') else None)) (C s)" 
   shows "
     (if I s then Some (E s) else None) = Some t \<Longrightarrow>
-    b s \<Longrightarrow> Some 0 \<le> T (\<lambda>s'. mm3 t (if I s' then Some (E s') else None)) (C s)"
+    b s \<Longrightarrow> Some 0 \<le> lst (\<lambda>s'. mm3 t (if I s' then Some (E s') else None)) (C s)"
  apply(cases "I s")
   subgoal apply simp
     using assms by auto
@@ -1875,28 +1872,28 @@ lemma transf:
 lemma  whileIET_rule':
   fixes E
   assumes 
-    "(\<And>s t t'. I s \<Longrightarrow>  b s \<Longrightarrow> Some 0 \<le> T (\<lambda>s'. mm3 (E s) (if I s' then Some (E s') else None)) (C s))" 
+    "(\<And>s t t'. I s \<Longrightarrow>  b s \<Longrightarrow> Some 0 \<le> lst (\<lambda>s'. mm3 (E s) (if I s' then Some (E s') else None)) (C s))" 
   "\<And>s. progress (C s)"
   "I s0" 
-shows "Some 0 \<le> T (\<lambda>x. if b x then None else mm3 (E s0) (if I x then Some (E x) else None)) (whileIET I E b C s0)" 
+shows "Some 0 \<le> lst (\<lambda>x. if b x then None else mm3 (E s0) (if I x then Some (E x) else None)) (whileIET I E b C s0)" 
   apply(rule whileIET_rule) apply(rule transf[where b=b]) using assms by auto  
    
 
 lemma 
-  assumes IS: "T (\<lambda>s. T (\<lambda>s'. if (s',s)\<in>R then I s' else None) (c s)) (SPECT (\<lambda>x. if b x then I x else None)) \<ge> Some 0" 
+  assumes IS: "lst (\<lambda>s. lst (\<lambda>s'. if (s',s)\<in>R then I s' else None) (c s)) (SPECT (\<lambda>x. if b x then I x else None)) \<ge> Some 0" 
   assumes wf: "wf R"
-  shows whileT_rule''_: "T (\<lambda>s. T (\<lambda>x. if b x then None else I x) (whileT b c s)) (SPECT I) \<ge> Some 0"
+  shows whileT_rule''_: "lst (\<lambda>s. lst (\<lambda>x. if b x then None else I x) (whileT b c s)) (SPECT I) \<ge> Some 0"
   using IS   unfolding  waux1[symmetric] unfolding  waux2[symmetric]  using whileT_rule''[OF _ _ _ wf]
   by blast
  
 
 lemma
   assumes "whileT b c s = r"
-  assumes IS[vcg_rules]: "\<And>s t'. I s = Some t' \<Longrightarrow> b s  \<Longrightarrow> T I (c s) \<ge> Some t'"
+  assumes IS[vcg_rules]: "\<And>s t'. I s = Some t' \<Longrightarrow> b s  \<Longrightarrow> lst I (c s) \<ge> Some t'"
     (*  "T (\<lambda>x. T I (c x)) (SPECT (\<lambda>x. if b x then I x else None)) \<ge> Some 0" *) 
   assumes "I s = Some t'"
   assumes wf: "wf {(y, x)|x M y. I x \<noteq> None \<and> b x \<and> c x = SPECT M \<and> M y \<noteq> None}"
-  shows whileT_rule': "T (\<lambda>x. if b x then None else I x) r \<ge> Some t'"
+  shows whileT_rule': "lst (\<lambda>x. if b x then None else I x) r \<ge> Some t'"
   using assms(1,3)
   unfolding whileT_def
 proof (induction arbitrary: t' rule: RECT_wf_induct[where R="{(y, x)|x M y. I x \<noteq> None \<and> b x \<and> c x = SPECT M \<and> M y \<noteq> None}"])
@@ -1922,9 +1919,9 @@ qed
 
 print_statement waux1
 lemma 
-  assumes IS: "T (\<lambda>s. T I (c s)) (SPECT (\<lambda>x. if b x then I x else None)) \<ge> Some 0" 
+  assumes IS: "lst (\<lambda>s. lst I (c s)) (SPECT (\<lambda>x. if b x then I x else None)) \<ge> Some 0" 
   assumes wf: "wf {(y, x)|x M y. I x \<noteq> None \<and> b x \<and> c x = SPECT M \<and> M y \<noteq> None}"
-  shows whileT_rule_: "T (\<lambda>s. T (\<lambda>x. if b x then None else I x) (whileT b c s)) (SPECT I) \<ge> Some 0"
+  shows whileT_rule_: "lst (\<lambda>s. lst (\<lambda>x. if b x then None else I x) (whileT b c s)) (SPECT I) \<ge> Some 0"
   using IS unfolding  waux1[symmetric] waux2[symmetric]  using whileT_rule[OF _ _ _ wf] by blast
 
 
@@ -1940,7 +1937,7 @@ subsubsection "Examples"
 lemma 
   assumes c: "c = (\<lambda>s. SPECT [s-1\<mapsto>1])" 
       and n: "S\<le>n"
-  shows ex4: "T (\<lambda>s. if s = 0 then Some (enat n) else None) (whileT (\<lambda>s. s>0) c (S::nat)) \<ge> Some 0"
+  shows ex4: "lst (\<lambda>s. if s = 0 then Some (enat n) else None) (whileT (\<lambda>s. s>0) c (S::nat)) \<ge> Some 0"
   apply(rule T_conseq4)
    apply(rule whileT_rule'''[where I="\<lambda>s. if s\<le>n then Some (s) else None" ])
       apply simp
@@ -1949,7 +1946,7 @@ lemma
     by(auto simp: mm2_def mm3_def one_enat_def)
   using n by (auto simp: mm3_Some_conv split: if_splits) 
 
-lemma Refinement_by_T: assumes "T Q m \<ge> Some 0"
+lemma Refinement_by_T: assumes "lst Q m \<ge> Some 0"
   shows "m \<le> SPECT Q"
   apply(simp add:  pw_le_iff )
   apply(cases m) 
@@ -1969,7 +1966,7 @@ lemma assumes "c = (\<lambda>s. SPECT [s-1\<mapsto>1])"
 lemma 
   assumes c: "c = (\<lambda>s. SPECT [s-1\<mapsto>1])" 
       and n: "S\<le>n"
-  shows "T (\<lambda>s. if s = 0 then Some (enat n) else None) (whileT (\<lambda>s. s>0) c (S::nat)) \<ge> Some 0"
+  shows "lst (\<lambda>s. if s = 0 then Some (enat n) else None) (whileT (\<lambda>s. s>0) c (S::nat)) \<ge> Some 0"
   apply(rule T_conseq4)
    apply(rule whileT_rule''[where I="\<lambda>s. if s\<le>n then Some (enat (n - s)) else None"
             and R="measure nat"])
@@ -1985,7 +1982,7 @@ term emb'
 lemma 
   assumes c: "c = (\<lambda>s. SPECT [s-1\<mapsto>1])" 
       and n: "S\<le>n"
-  shows "T (\<lambda>s. if s = 0 then Some (enat n) else None) (whileT (\<lambda>s. s>0) c (S::nat)) \<ge> Some 0"
+  shows "lst (\<lambda>s. if s = 0 then Some (enat n) else None) (whileT (\<lambda>s. s>0) c (S::nat)) \<ge> Some 0"
   apply(rule T_conseq4)
    apply(rule whileT_rule[where I="\<lambda>s. if s\<le>n then Some (enat (n - s)) else None"])
       apply simp
@@ -2000,7 +1997,7 @@ lemma
 
 lemma                                       (* hmmm *)
   assumes c: "c = (\<lambda>s. SPECT (\<lambda>s'. if s'<s \<and> even s then Some C else None))"  
-  shows "T (\<lambda>s. if s = 0 then Some \<infinity> else None) (whileT (\<lambda>s. s>0) c (S::nat)) \<ge> Some 0"
+  shows "lst (\<lambda>s. if s = 0 then Some \<infinity> else None) (whileT (\<lambda>s. s>0) c (S::nat)) \<ge> Some 0"
   apply(rule T_conseq4)
    apply(rule whileT_rule[where I="\<lambda>s. Some \<infinity>"])
       apply simp
@@ -2011,13 +2008,13 @@ lemma                                       (* hmmm *)
   by (auto split: if_splits)
 
 
-lemma T_specifies_I: "T Q m \<ge> Some 0 \<Longrightarrow> (m \<le> SPECT Q)"
+lemma T_specifies_I: "lst Q m \<ge> Some 0 \<Longrightarrow> (m \<le> SPECT Q)"
   unfolding T_pw apply (cases m) apply (auto simp: miiFailt le_fun_def mii_alt mm2_def split: option.splits)
   subgoal for M x apply(cases "Q x"; cases "M x") apply (auto split: if_splits)
     apply force+ done
   done
 
-lemma T_specifies_rev: "(m \<le> SPECT Q) \<Longrightarrow> T Q m \<ge> Some 0" 
+lemma T_specifies_rev: "(m \<le> SPECT Q) \<Longrightarrow> lst Q m \<ge> Some 0" 
   unfolding T_pw apply (cases m)
   subgoal by auto
    apply (auto simp: miiFailt le_fun_def mii_alt mm2_def split: option.splits)
@@ -2026,13 +2023,13 @@ lemma T_specifies_rev: "(m \<le> SPECT Q) \<Longrightarrow> T Q m \<ge> Some 0"
   subgoal by (metis leD less_option_Some) 
   done
 
-lemma T_specifies: "T Q m \<ge> Some 0 = (m \<le> SPECT Q)"
+lemma T_specifies: "lst Q m \<ge> Some 0 = (m \<le> SPECT Q)"
   using T_specifies_I T_specifies_rev by metis
 
 thm whileT_rule''
 lemma                                       (* hmmm *)
   assumes c[vcg_rules]: "\<And>s. c s \<le> SPECT (\<lambda>s'. if s'<s \<and> even s then Some C else None)"  
-  shows "T (\<lambda>s. if s \<le> 0 then Some \<infinity> else None) (whileT (\<lambda>s. s>0) c (S::nat)) \<ge> Some 0"
+  shows "lst (\<lambda>s. if s \<le> 0 then Some \<infinity> else None) (whileT (\<lambda>s. s>0) c (S::nat)) \<ge> Some 0"
   apply(rule  whileT_rule''[where I="\<lambda>s. Some \<infinity>" and R="{(x, y). x < y}", THEN T_conseq4])
       apply simp 
      apply(rule T_conseq4)
@@ -2048,28 +2045,28 @@ print_statement whileT_rule''
 
 lemma  whileTI_rule[vcg_rules]:
   assumes 
-      "\<And>s t'. I s = Some t' \<Longrightarrow> b s \<Longrightarrow> Some t' \<le> T (\<lambda>s'. if (s', s) \<in> R then I s' else None) (c s)"
+      "\<And>s t'. I s = Some t' \<Longrightarrow> b s \<Longrightarrow> Some t' \<le> lst (\<lambda>s'. if (s', s) \<in> R then I s' else None) (c s)"
     and "I s = Some t'"
     and "wf R"
-  shows "Some t' \<le> T (\<lambda>x. if b x then None else I x) (whileTI I R b c s)"
+  shows "Some t' \<le> lst (\<lambda>x. if b x then None else I x) (whileTI I R b c s)"
   unfolding   whileTI_def
   apply(rule whileT_rule''[where I=I and R=R])
   apply simp apply fact+ done
  
 thm vcg_rules
 lemma                                       (* hmmm *)
-  assumes c[vcg_rules]: "\<And>s. Some 0 \<le> T (\<lambda>s'. if s' < s \<and> even s then Some C else None) (c s)"  
-  shows "T (\<lambda>s. if s \<le> 0 then Some \<infinity> else None) (whileTI (\<lambda>s. Some \<infinity>) {(x, y). x < y} (\<lambda>s. s>0) c (S::nat)) \<ge> Some 0"
+  assumes c[vcg_rules]: "\<And>s. Some 0 \<le> lst (\<lambda>s'. if s' < s \<and> even s then Some C else None) (c s)"  
+  shows "lst (\<lambda>s. if s \<le> 0 then Some \<infinity> else None) (whileTI (\<lambda>s. Some \<infinity>) {(x, y). x < y} (\<lambda>s. s>0) c (S::nat)) \<ge> Some 0"
   apply vcg  
      apply (auto split: if_splits)   by(fact wf) 
 
 
 
 lemma   fixes n :: nat
-  assumes [vcg_rules]: "T (\<lambda>s. if s \<le> n then Some 1 else None) f \<ge> Some 0"
-   and  c[vcg_rules]: "\<And>s. Some 0 \<le> T (\<lambda>s'. if s' < s then Some (enat C) else None) (c s)"
+  assumes [vcg_rules]: "lst (\<lambda>s. if s \<le> n then Some 1 else None) f \<ge> Some 0"
+   and  c[vcg_rules]: "\<And>s. Some 0 \<le> lst (\<lambda>s'. if s' < s then Some (enat C) else None) (c s)"
    and C: "C>0"
-  shows "T (\<lambda>s. if s \<le> 0 then Some (1+C*n) else None) (
+  shows "lst (\<lambda>s. if s \<le> 0 then Some (1+C*n) else None) (
         do { n \<leftarrow> f;
              whileT (\<lambda>s. s>0) c n }) \<ge> Some 0"
     (* note that n is bound from the outside ! *)
@@ -2089,10 +2086,10 @@ lemma   fixes n :: nat
 
 
 lemma   fixes n :: nat
-  assumes [vcg_rules]: "T (\<lambda>s. if s \<le> n then Some 1 else None) f \<ge> Some 0"
-   and  c[vcg_rules]: "\<And>s. Some 0 \<le> T (\<lambda>s'. if s' < s then Some (enat C) else None) (c s)"
+  assumes [vcg_rules]: "lst (\<lambda>s. if s \<le> n then Some 1 else None) f \<ge> Some 0"
+   and  c[vcg_rules]: "\<And>s. Some 0 \<le> lst (\<lambda>s'. if s' < s then Some (enat C) else None) (c s)"
    and C: "C>0"
-  shows "T (\<lambda>s. if s \<le> 0 then Some (1+C*n) else None) (
+  shows "lst (\<lambda>s. if s \<le> 0 then Some (1+C*n) else None) (
         do { n \<leftarrow> f;
              whileTI (\<lambda>s. if s\<le>n then Some (1+C*(enat (n-s))) else None)  {(x, y). x < y}  (\<lambda>s. s>0) c n }) \<ge> Some 0" 
     (* note that n in the Invariant is bound from the inside, very much in contrast to the example above! ! *)
@@ -2115,7 +2112,7 @@ lemma dont_care_about_runtime_as_long_as_it_terminates:
         * the cost C of of the loop body (decrementing s) may even be \<infinity>
         * the starting state S is also arbitrary *)
   assumes c: "c = (\<lambda>s. SPECT [s-1\<mapsto>C])"
-  shows "T (\<lambda>s. if s = 0 then Some \<infinity> else None) (whileT (\<lambda>s. s>0) c (S::nat)) \<ge> Some 0"
+  shows "lst (\<lambda>s. if s = 0 then Some \<infinity> else None) (whileT (\<lambda>s. s>0) c (S::nat)) \<ge> Some 0"
   apply(rule T_conseq4)
    apply(rule whileT_rule[where I="\<lambda>s. Some \<infinity>"])
       apply simp
@@ -2133,7 +2130,7 @@ lemma "SPECT  [r\<mapsto>i] \<le> SPECT [f\<mapsto>j] \<longleftrightarrow> ((r 
    apply simp unfolding le_fun_def by simp
 
 
-abbreviation "TTT == T"
+abbreviation "TTT == lst"
  
 
  
@@ -2145,7 +2142,7 @@ abbreviation "TTT == T"
   subsection "weakest precondition & strongest postcondition"
 
 
-definition "wp Q c = (\<lambda>s. T Q (c s))"
+definition "wp Q c = (\<lambda>s. lst Q (c s))"
 
 
 lemma "FAILT \<le> SPECT Q" apply simp oops
@@ -2156,7 +2153,7 @@ lemma "(\<forall>s. P s \<longrightarrow> (c s) \<le> SPECT Q) \<longleftrightar
   subgoal unfolding emb'_def wp_def le_fun_def apply (auto simp: T_specifies[symmetric]) by metis
   done
 
-  thm T_def
+  thm lst_def
 
 definition "spl P c s s' = None"
 
@@ -2229,7 +2226,7 @@ lemma sp_refines: "(\<forall>s. P s \<longrightarrow> (c s) \<le> SPECT Q) \<lon
   by(auto intro: sp_refines1 sp_refines2) 
 
 lemma wpI: "(\<And>s s'. P s \<le> mii Q (c s) s' ) \<Longrightarrow> P \<le> wp Q c"
-  unfolding wp_def T_def apply(auto simp add: le_fun_def)
+  unfolding wp_def lst_def apply(auto simp add: le_fun_def)
   apply(rule Inf_greatest) by auto
 
 lemma f: "a + b \<le> a' \<Longrightarrow> \<not> a' < a \<Longrightarrow> b \<le> a' - (a::enat)"
@@ -2251,7 +2248,7 @@ lemma Someplus_mii_conv: "Someplus (M s) t s \<le> Q \<longleftrightarrow> t \<l
 
 lemma wpD: assumes "P \<le> wp Q c" 
   shows "(\<And>s s'. P s \<le> mii Q (c s) s' )"
-  using assms unfolding wp_def T_def by(auto simp add: le_fun_def le_Inf_iff) 
+  using assms unfolding wp_def lst_def by(auto simp add: le_fun_def le_Inf_iff) 
  
 
 lemma sp_wp: "(sp P c \<le> SPECT Q) \<longleftrightarrow> P \<le> wp Q c"
@@ -2281,7 +2278,7 @@ lemma "wp Q (\<lambda>_. RETURNT x) = (\<lambda>_. Q x)"
   unfolding wp_def T_RETURNT by simp
 
 lemma "wp Q (\<lambda>s. SPECT (f s))  = foo"
-  unfolding wp_def unfolding T_def mii_alt apply(rule)
+  unfolding wp_def unfolding lst_def mii_alt apply(rule)
     apply (simp add:  ) oops
     
 
@@ -2420,8 +2417,7 @@ method_setup refine_vcg =
 
 
 
-
-hide_const T
+ 
 
 
 
